\label{ExercisesforAppRatExpEqus}

In Exercises \ref{ratsimpfirst} - \ref{ratsimplast}, perform the indicated operations and simplify.

\begin{tasks}(2)

\task $\dfrac{x^2-9}{x^2} \cdot \dfrac{3x}{x^2-x-6}$\vphantom{$\dfrac{4y-y^2}{2y+1} \div \dfrac{y^2-16}{2y^2-5y-3}$}\label{ratsimpfirst}
\task $\dfrac{t^2-2t}{t^2+1} \div (3t^2 - 2t - 8)$\vphantom{$\dfrac{4y-y^2}{2y+1} \div \dfrac{y^2-16}{2y^2-5y-3}$}
\task $\dfrac{4y-y^2}{2y+1} \div \dfrac{y^2-16}{2y^2-5y-3}$

\task  $\dfrac{x}{3x-1} - \dfrac{1-x}{3x-1}$\vphantom{$\dfrac{2-y}{3y} - \dfrac{1-y}{3y} + \dfrac{y^2-1}{3y}$}
\task  $\dfrac{2}{w-1} - \dfrac{w^2+1}{w-1}$\vphantom{$\dfrac{2-y}{3y} - \dfrac{1-y}{3y} + \dfrac{y^2-1}{3y}$}
\task  $\dfrac{2-y}{3y} - \dfrac{1-y}{3y} + \dfrac{y^2-1}{3y}$
\task  $b+ \dfrac{1}{b-3} - 2$\vphantom{$\dfrac{m^2}{m^2-4} + \dfrac{1}{2-m}$}
\task  $\dfrac{2x}{x-4} - \dfrac{1}{2x+1}$\vphantom{$\dfrac{m^2}{m^2-4} + \dfrac{1}{2-m}$}
\task  $\dfrac{m^2}{m^2-4} + \dfrac{1}{2-m}$

\task $\dfrac{\dfrac{2}{x} - 2}{x-1}$\vphantom{$\dfrac{\dfrac{1}{x+h} - \dfrac{1}{x}}{h}$}
\task $\dfrac{\dfrac{3}{2-h} - \dfrac{3}{2}}{h}$\vphantom{$\dfrac{\dfrac{1}{x+h} - \dfrac{1}{x}}{h}$}
\task $\dfrac{\dfrac{1}{x+h} - \dfrac{1}{x}}{h}$


\task  $3w^{-1} - (3w)^{-1}$
\task  $-2y^{-1}  + 2(3-y)^{-2}$
\task  $3(x-2)^{-1} - 3x(x-2)^{-2}$

 
\task $\dfrac{t^{-1} + t^{-2}}{t^{-3}}$  
\task $\dfrac{2(3+h)^{-2} - 2(3)^{-2}}{h}$ \vphantom{$\dfrac{t^{-1} + t^{-2}}{t^{-3}}$}
\task $\dfrac{(7-x-h)^{-1} - (7-x)^{-1}}{h}$ \vphantom{$\dfrac{t^{-1} + t^{-2}}{t^{-3}}$} \label{ratsimplast}

\end{tasks}

In Exercises \ref{rateqnfirst} - \ref{rateqnlast}, find all real solutions.  Be sure to check for extraneous solutions.

\begin{tasks}[resume](2)

\task $\dfrac{x}{5x + 4} = 3$\vphantom{$\dfrac{1}{w + 3} + \dfrac{1}{w - 3} = \dfrac{w^{2} - 3}{w^{2} - 9}$} \label{rateqnfirst}
\task $\dfrac{3y - 1}{y^{2} + 1} = 1$\vphantom{$\dfrac{1}{w + 3} + \dfrac{1}{w - 3} = \dfrac{w^{2} - 3}{w^{2} - 9}$}
\task $\dfrac{1}{w + 3} + \dfrac{1}{w - 3} = \dfrac{w^{2} - 3}{w^{2} - 9}$


\task $\dfrac{2x + 17}{x + 1} = x + 5$\vphantom{$\dfrac{-y^{3} + 4y}{y^{2} - 9} = 4y$}
\task $\dfrac{t^{2} - 2t + 1}{t^{3} + t^{2} - 2t} = 1$\vphantom{$\dfrac{-y^{3} + 4y}{y^{2} - 9} = 4y$}
\task $\dfrac{-y^{3} + 4y}{y^{2} - 9} = 4y$  

\task $w + \sqrt{3} = \dfrac{3w - w^3}{w - \sqrt{3}}$\vphantom{ $\dfrac{x^2}{(1 + x\sqrt{3})^2} = 3$}
\task $\dfrac{2}{x\sqrt{2} - 1}  - 1 = \dfrac{3}{x \sqrt{2} + 1}$\vphantom{ $\dfrac{x^2}{(1 + x\sqrt{3})^2} = 3$}
\task $\dfrac{x^2}{(1 + x\sqrt{3})^2} = 3$ \label{rateqnlast}

\end{tasks}

In Exercises \ref{absratfirst} - \ref{absratlast}, use Theorem \ref{absvalequality} along with the techniques in this section to find all real solutions.

\begin{tasks}[resume](2)

\task $\left|\dfrac{3n}{n-1}  \right| = 3$\vphantom{$\left| \dfrac{2t}{4-t^2}\right| = \left|\dfrac{2}{t-2}\right|$} \label{absratfirst}
\task $\left| \dfrac{2x}{x^2-1}\right| = 2$\vphantom{$\left| \dfrac{2t}{4-t^2}\right| = \left|\dfrac{2}{t-2}\right|$}
\task $\left| \dfrac{2t}{4-t^2}\right| = \left|\dfrac{2}{t-2}\right|$ \label{absratlast}

\end{tasks}

In Exercises \ref{solveratcalcfirst} - \ref{solveratcalclast}, find all real solutions and use a calculator to approximate your answers, rounded to two decimal places.

\begin{tasks}[resume](2)

\task $2.41 = \dfrac{0.08}{4 \pi R^2}$ \label{solveratcalcfirst}
\task $\dfrac{x^2}{(2.31 -x)^2} = 0.04$
\task $1 - \dfrac{6.75 \times 10^{16}}{c^2} = \dfrac{1}{4}$ \label{solveratcalclast}

\end{tasks}

In Exercises \ref{litrateqnfirst} - \ref{litrateqnlast}, solve the given equation for the indicated variable.

\begin{tasks}[resume](2)

\task Solve for $y$:  $\dfrac{1-2y}{y+3} = x$ \label{litrateqnfirst}

\task Solve for $y$: $x = 3 - \dfrac{2}{1-y}$ \vphantom{$\dfrac{1-2y}{y+3} = x$}

\task\hspace{-0.1in}\footnote{Recall: subscripts on variables have no intrinsic mathematical meaning; they're just used to distinguish one variable from another.  In other words, treat quantities like `$V_{\text{\tiny $1$}}$' and `$V_{\text{\tiny $2$}}$'  as two different variables as you would `$x$' and `$y$.'}Solve for $T_{\text{\tiny $2$}}$:  $\dfrac{V_{\text{\tiny $1$}}}{T_{\text{\tiny $1$}}} = \dfrac{V_{\text{\tiny $2$}}}{T_{\text{\tiny $2$}}}$


\task  Solve for $t_{\text{\tiny $0$}}$:  $\dfrac{t_{\text{\tiny $0$}}}{1-t_{\text{\tiny $0$}}t_{\text{\tiny $1$}}} = 2$ 


\task  Solve for $x$:  $\dfrac{1}{x - v_{\text{\tiny $r$}}} + \dfrac{1}{x + v_{\text{\tiny $r$}}} = 5$

\task Solve for $R$:  $P = \dfrac{25R}{(R+4)^2}$ \label{litrateqnlast}

\end{tasks}

\clearpage

\subsection{Answers}

\begin{tasks}(2)

\task $\dfrac{3(x+3)}{x(x+2)}$, $x \neq 3$\vphantom{$-\dfrac{y(y-3)}{y+4}$, $y \neq -\dfrac{1}{2}, 3, 4$}
\task $\dfrac{t}{(3t+4)(t^2+1)}$, $t \neq 2$\vphantom{$-\dfrac{y(y-3)}{y+4}$, $y \neq -\dfrac{1}{2}, 3, 4$}
\task $-\dfrac{y(y-3)}{y+4}$, $y \neq -\dfrac{1}{2}, 3, 4$ 

\task  $\dfrac{2x-1}{3x-1}$
\task  $-w-1$, $w \neq 1$\vphantom{$\dfrac{2x-1}{3x-1}$}
\task  $\dfrac{y}{3}$, $y \neq 0$\vphantom{$\dfrac{2x-1}{3x-1}$}
\task  $\dfrac{b^2-5b+7}{b-3}$\vphantom{$\dfrac{4x^2+x+4}{(x-4)(2x+1)}$}
\task  $\dfrac{4x^2+x+4}{(x-4)(2x+1)}$
\task  $\dfrac{m+1}{m+2}$, $m \neq 2$\vphantom{$\dfrac{4x^2+x+4}{(x-4)(2x+1)}$}
\task $-\dfrac{2}{x}$, $x \neq 1$\vphantom{$\dfrac{3}{4-2h}$, $h \neq 0$}
\task $\dfrac{3}{4-2h}$, $h \neq 0$
\task $-\dfrac{1}{x(x+h)}$, $h \neq 0$\vphantom{$\dfrac{3}{4-2h}$, $h \neq 0$}

\task  $\dfrac{8}{3w}$\vphantom{$-\dfrac{2(y^2-7y+9)}{y(y-3)^2}$}
\task  $-\dfrac{2(y^2-7y+9)}{y(y-3)^2}$
\task  $-\dfrac{6}{(x-2)^2}$\vphantom{$-\dfrac{2(y^2-7y+9}{y(y-3)^2}$}

\task $t^2+t$, $t \neq 0$\vphantom{$\dfrac{1}{(7-x)(7-x-h)}$, $h \neq 0$}  
\task $-\dfrac{2(h+6)}{9(h+3)^2}$, $h \neq 0$ \vphantom{$\dfrac{1}{(7-x)(7-x-h)}$, $h \neq 0$}
\task $\dfrac{1}{(7-x)(7-x-h)}$, $h \neq 0$ 


\task $x = -\dfrac{6}{7}$
\task $y = 1, 2$ \vphantom{$x = -\dfrac{6}{7}$}
\task $w = -1$ \vphantom{$x = -\dfrac{6}{7}$}
\task $x=-6, 2$
\task No solution.
\task $y = 0, \pm 2\sqrt{2}$  


\task $w = -\sqrt{3}, -1$\vphantom{$x = -\dfrac{\sqrt{3}}{2}, -\dfrac{\sqrt{3}}{4}$}
\task $x = -\dfrac{3\sqrt{2}}{2}, \sqrt{2}$\vphantom{$x = -\dfrac{\sqrt{3}}{2}, -\dfrac{\sqrt{3}}{4}$}
\task $x = -\dfrac{\sqrt{3}}{2}, -\dfrac{\sqrt{3}}{4}$

\task $n = \dfrac{1}{2}$\vphantom{$x = \dfrac{1 \pm \sqrt{5}}{2}, \dfrac{-1 \pm \sqrt{5}}{2}$}
\task $x = \dfrac{1 \pm \sqrt{5}}{2}, \dfrac{-1 \pm \sqrt{5}}{2}$
\task $t = -1$\vphantom{$x = \dfrac{1 \pm \sqrt{5}}{2}, \dfrac{-1 \pm \sqrt{5}}{2}$}


\task $R = \pm \sqrt{\dfrac{0.08}{9.64 \pi}} \approx \pm 0.05$ 
\task! $x = -\dfrac{231}{400} \approx -0.58$, $x = \dfrac{77}{200} \approx 0.38$ \vphantom{ $R = \pm \sqrt{\dfrac{0.08}{9.64 \pi}} \approx \pm 0.05$ }

\task! $c = \pm \sqrt{\dfrac{4 \cdot 6.75 \times 10^{16}}{3}} = \pm 3.00 \times 10^{8}$ (You actually didn't 
\textit{need} a calculator for this!)


\task! $y = \dfrac{1 - 3x}{x+2}$, $y \neq -3$, $x \neq -2$

\task! $y = \dfrac{x-1}{x-3}$, $y \neq 1$, $x \neq 3$

\task! $T_{\text{\tiny $2$}} = \dfrac{V_{\text{\tiny $2$}}T_{\text{\tiny $1$}}}{V_{\text{\tiny $1$}}}$, $T_{\text{\tiny $1$}} \neq 0, T_{\text{\tiny $2$}} \neq 0, V_{\text{\tiny $1$}} \neq 0$


\task!  $t_{\text{\tiny $0$}} = \dfrac{2}{2t_{\text{\tiny $1$}} + 1}$, $t_{\text{\tiny $1$}} \neq -\dfrac{1}{2}$\vphantom{$T_{\text{\tiny $2$}} = \dfrac{V_{\text{\tiny $2$}}T_{\text{\tiny $1$}}}{V_{\text{\tiny $1$}}}$, $T_{\text{\tiny $1$}}, T_{\text{\tiny $2$}}, V_{\text{\tiny $1$}} \neq 0$}
\task!  $x = \dfrac{1 \pm \sqrt{25v_{\text{\tiny $r$}}^2+1}}{5}$, $x \neq \pm v_{\text{\tiny $r$}}$.

\task! $R= \dfrac{-(8P-25) \pm \sqrt{(8P-25)^2 - 64P^2}}{2P} = \dfrac{(25-8P) \pm 5 \sqrt{25-16P}}{2P}$, $P \neq 0$, $R \neq -4$

\end{tasks}
