\label{ExercisesforAppRadEqus}

In Exercises \ref{simpradfirst} - \ref{simpradlast}, perform the indicated operations and simplify.

\begin{tasks}(2)
\task   $\sqrt{9x^2}$ \label{simpradfirst}

\task   $\sqrt[3]{8t^3}$

\task   $\sqrt{50y^6}$

\task  $\sqrt{4t^2 + 4t + 1}$

\task  $\sqrt{w^2 - 16w + 64}$

\task  $\sqrt{(\sqrt{12x} - \sqrt{3x})^2+1}$

\task  $\sqrt{\dfrac{c^2 - v^2}{c^2}}$\vphantom{$\sqrt[3]{\dfrac{24 \pi r^5}{L^3}}$}

\task  $\sqrt[3]{\dfrac{24 \pi r^5}{L^3}}$

\task   $\sqrt[4]{\dfrac{32 \pi \varepsilon^8}{\rho^{12}}}$ \vphantom{$\sqrt[3]{\dfrac{24 \pi r^5}{L^3}}$}   

\task $\sqrt{x} - \dfrac{x+1}{\sqrt{x}}$\vphantom{$3 \sqrt{1-t^2} + 3t\left(\dfrac{1}{2 \sqrt{1-t^2}}\right)(-2t)$}

\task! $3 \sqrt{1-t^2} + 3t\left(\dfrac{1}{2 \sqrt{1-t^2}}\right)(-2t)$

\task! $2 \sqrt[3]{1-z} + 2z \left(\dfrac{1}{3 \left(\sqrt[3]{1-z}\right)^2}\right)(-1)$\vphantom{$\dfrac{3}{\sqrt[3]{2x-1}} + (3x)\left(-\dfrac{1}{3 \left(\sqrt[3]{2x-1} \right)^4}\right)(2)$}


\task!  $\dfrac{3}{\sqrt[3]{2x-1}} + (3x)\left(-\dfrac{1}{3 \left(\sqrt[3]{2x-1} \right)^4}\right)(2)$  \label{simpradlast}

\end{tasks}



In Exercises \ref{algineqexfirst} - \ref{algineqexlast}, find all real solutions.

\begin{tasks}[resume](2)

\task  $(2x+1)^3 + 8 = 0$ \label{algineqexfirst} \vphantom{ $\dfrac{1}{1 + 2t^3} = 4$}
\task $\dfrac{(1-2y)^{4}}{3} = 27$ \vphantom{ $\dfrac{1}{1 + 2t^3} = 4$}
\task  $\dfrac{1}{1 + 2t^3} = 4$ 

\task $\sqrt{3x+1} = 4$
\task $5 - \sqrt[3]{t^2+1} = 1$
\task $x+1 = \sqrt{3x+7}$ % $x=3$     

\task  $y + \sqrt{3y+10} = -2$ % $y=-3$
\task  $3t+\sqrt{6-9t}=2$ % $x = -\dfrac{1}{3}, \dfrac{2}{3}$
\task $2x - 1 = \sqrt{x + 3}$ % $x = \dfrac{5 + \sqrt{57}}{8}$


\task $w = \sqrt[4]{12-w^2}$
\task $\sqrt{x - 2} + \sqrt{x - 5} = 3$ % $x = 6$
\task $\sqrt{2x+1} = 3 + \sqrt{4-x}$  \label{algineqexlast} % $x = 4$

\end{tasks}

In Exercises \ref{radliteqnfirst} - \ref{radliteqnlast}, solve each equation for the indicated variable.  Assume all quantities represent positive real numbers.

\begin{tasks}[resume](2)

\task Solve for $h$:  $I = \dfrac{bh^3}{12}$. \vphantom{$I_{\text{\tiny $0$}} = \dfrac{5\sqrt{3} a^4}{16}$} \label{radliteqnfirst}

\task Solve for $a$:  $I_{\text{\tiny $0$}} = \dfrac{5\sqrt{3} a^4}{16}$

\task Solve for $g$:  $T = 2\pi \sqrt{\dfrac{L}{g}}$

\task Solve for $v$:   $L = L_{\text{\tiny $0$}} \sqrt{1 - \dfrac{v^2}{c^2}}$. \vphantom{$T = 2\pi \sqrt{\dfrac{L}{g}}$} \label{radliteqnlast}

\end{tasks}

In Exercises \ref{rationalizefirst} - \ref{rationalizelast}, rationalize the numerator or denominator, and simplify.


\begin{tasks}[resume](2)

\task   $\dfrac{4}{3 - \sqrt{2}}$ \vphantom{$\dfrac{7}{\sqrt[3]{12x^7}}$} \label{rationalizefirst}

\task  $\dfrac{7}{\sqrt[3]{12x^7}}$

\task   $\dfrac{\sqrt{x} - \sqrt{c}}{x - c}$ \vphantom{$\dfrac{7}{\sqrt[3]{12x^7}}$}


\task  $\dfrac{\sqrt{2x+2h+1} - \sqrt{2x+1}}{h}$ 

\task  $\dfrac{\sqrt[3]{x+1} - 2}{x- 7}$                                          

\task  $\dfrac{\sqrt[3]{x+h} - \sqrt[3]{x}}{h}$  \label{rationalizelast}

\end{tasks}

\clearpage

\subsection{Answers}

\begin{tasks}(3)

\task   $3|x|$ 

\task   $2t$

\task   $5|y^3|\sqrt{2}$

\task  $|2t+1|$

\task  $|w-8|$

\task  $\sqrt{3x+1}$

\task $\dfrac{\sqrt{c^2-v^2}}{|c|}$ \vphantom{$\dfrac{2 \varepsilon^2 \sqrt[4]{2\pi}}{|\rho^3|}$ }

\task $\dfrac{2r \sqrt[3]{3 \pi r^2}}{L}$ \vphantom{$\dfrac{2 \varepsilon^2 \sqrt[4]{2\pi}}{|\rho^3|}$ }

\task  $\dfrac{2 \varepsilon^2 \sqrt[4]{2\pi}}{|\rho^3|}$ 


\task  $-\dfrac{1}{\sqrt{x}}$ \vphantom{$\dfrac{3-6t^2}{\sqrt{1-t^2}}$}

\task  $\dfrac{3-6t^2}{\sqrt{1-t^2}}$
\task  $\dfrac{6-8z}{3 (\sqrt[3]{1-z})^2}$


\task  $\dfrac{4x-3}{(2x-1)\sqrt[3]{2x-1}}$  


\task  $x = -\dfrac{3}{2}$ \vphantom{$t = -\dfrac{\sqrt[3]{3}}{2}$}
\task $y = -1, 2$ \vphantom{$t = -\dfrac{\sqrt[3]{3}}{2}$}
\task  $t = -\dfrac{\sqrt[3]{3}}{2}$ 

\task $x = 5$
\task $t = \pm 3 \sqrt{7}$
\task $x=3$     


\task  $y=-3$ \vphantom{$x = \dfrac{5 + \sqrt{57}}{8}$}
\task  $t = -\dfrac{1}{3}, \dfrac{2}{3}$ \vphantom{$x = \dfrac{5 + \sqrt{57}}{8}$}
\task $x = \dfrac{5 + \sqrt{57}}{8}$

\task $w = \sqrt{3}$
\task $x = 6$
\task $x = 4$


\task $h = \sqrt[3]{\dfrac{12I}{b}}$ \vphantom{ $a = \dfrac{2 \sqrt[4]{I_{\text{\tiny $0$}}}}{\sqrt[4]{5\sqrt{3}}}$}

\task  $a = \dfrac{2 \sqrt[4]{I_{\text{\tiny $0$}}}}{\sqrt[4]{5\sqrt{3}}}$
\task $g = \dfrac{4 \pi^2 L}{T^2}$ \vphantom{$v = \dfrac{c \sqrt{L_{\text{\tiny $0$}}^2 - L^2}}{L_{\text{\tiny $0$}}}$}

\task $v = \dfrac{c \sqrt{L_{\text{\tiny $0$}}^2 - L^2}}{L_{\text{\tiny $0$}}}$  

\task   $\dfrac{12 + 4\sqrt{2}}{7}$ \vphantom{$\dfrac{7 \sqrt[3]{18x^2}}{6x^3}$} 

\task  $\dfrac{7 \sqrt[3]{18x^2}}{6x^3}$

\task   $\dfrac{1}{\sqrt{x}+ \sqrt{c}}$ \vphantom{$\dfrac{7 \sqrt[3]{18x^2}}{6x^3}$}

\task!  $\dfrac{2}{\sqrt{2x+2h+1} + \sqrt{2x+1}}$ \vphantom{$\dfrac{1}{(\sqrt[3]{x+h})^2 + \sqrt[3]{x+h}\sqrt[3]{x} + (\sqrt[3]{x})^2}$}                                 

\task  $\dfrac{1}{(\sqrt[3]{x+1})^2 + 2\sqrt[3]{x+1} + 4}$   \vphantom{$\dfrac{1}{(\sqrt[3]{x+h})^2 + \sqrt[3]{x+h}\sqrt[3]{x} + (\sqrt[3]{x})^2}$}                                 

\task!  $\dfrac{1}{(\sqrt[3]{x+h})^2 + \sqrt[3]{x+h}\sqrt[3]{x} + (\sqrt[3]{x})^2}$

\end{tasks}
