\label{ExercisesforAppAbsValEqIneq}

In Exercises \ref{solveabsvalequfirst} - \ref{solveabsvalequlast}, solve the equation.

\begin{tasks}(2)
\task  $|x| = 6$ \label{solveabsvalequfirst} 
\task $|3t-1| = 10$
\task $|4-w| = 7$
\task  $4 - |y| = 3$
\task $2|5m+1| - 3 = 0$
\task $|7x-1| + 2 = 0$
\task $\dfrac{5 - |x|}{2} = 1$ \vphantom{$\dfrac{|2x+1| - 3}{4} = \dfrac{1}{2} - |2x+1|$}
\task $\dfrac{2}{3} |5-2w| - \dfrac{1}{2} = 5$ \vphantom{$\dfrac{|2x+1| - 3}{4} = \dfrac{1}{2} - |2x+1|$}
\task $|3t - \sqrt{2}| + 4 = 6$ 
\task $\dfrac{|2v+1| - 3}{4} = \dfrac{1}{2} - |2v+1|$
\task $|2x+1| = \dfrac{|2x+1| - 3}{2}$\vphantom{$\dfrac{|2v+1| - 3}{4} = \dfrac{1}{2} - |2v+1|$}
\task $\dfrac{|3-2y|+ 4}{2} = 2 - |3-2y|$\vphantom{$\dfrac{|2v+1| - 3}{4} = \dfrac{1}{2} - |2v+1|$}
\task $|3t - 2| = |2t + 7|$  
\task $|3x+1| = |4x|$
\task $|1-\sqrt{2} y| = |y+1|$
\task  $|4-x| - |x+2| = 0$
\task $|2-5z| = 5 |z+1|$
\task $\sqrt{3}|w-1| = 2|w+1|$ \label{solveabsvalequlast}
\end{tasks}


In Exercises \ref{solveinequabsquadfirst} - \ref{solveinequabsquadlast}, solve the inequality.  Write your answer using interval notation. 

\begin{tasks}[resume](2)
\task $|3x - 5| \leq 4$ \label{solveinequabsquadfirst}
\task $|7t + 2| > 10$
\task $|2w+1| - 5 < 0$   
\task $|2-y| - 4 \geq -3$
\task $|3z+5| + 2 < 1$   
\task $2|7-v| +4 > 1$
\task $3 - |x+\sqrt{5}| < -3$
\task $|5t| \leq |t|+3$   
\task $|w-3| < |3-w|$
\task  $2 \leq |4-y| < 7$ 
\task $1 < |2w - 9| \leq 3$ 
\task  $3 > 2|\sqrt{3} - x| > 1$ \label{solveinequabsquadlast}
\task!  With help from your classmates, solve:

\begin{enumerate}[label=(\alph*)]
\item  $|5 - |2x-3|| = 4$
\item   $|5 - |2x-3|| < 4$
\end{enumerate}

\end{tasks}


\newpage

\subsection{Answers}

\begin{tasks}(2)
\task  $x = -6$ or $x=6$ \vphantom{$t = -3$ or $t= \dfrac{11}{3}$}
\task $t = -3$ or $t= \dfrac{11}{3}$
\task $w = -3$ or $w= 11$ \vphantom{$t = -3$ or $t= \dfrac{11}{3}$}
\task  $y = -1$ or $y= 1$\vphantom{$m=-\dfrac{1}{2}$ or $m= \dfrac{1}{10}$}
\task $m=-\dfrac{1}{2}$ or $m= \dfrac{1}{10}$
\task No solution\vphantom{$m=-\dfrac{1}{2}$ or $m= \dfrac{1}{10}$}
\task  $x=-3$ or $x= 3$\vphantom{$t = \dfrac{\sqrt{2} \pm 2}{3}$}
\task $w = -\dfrac{13}{8}$ or $w= \dfrac{53}{8}$\vphantom{$t = \dfrac{\sqrt{2} \pm 2}{3}$}
\task $t = \dfrac{\sqrt{2} \pm 2}{3}$
\task $v = -1$ or $v = 0$ \vphantom{$y = \dfrac{3}{2}$}
\task  No solution\vphantom{$y = \dfrac{3}{2}$}
\task  $y = \dfrac{3}{2}$
\task $t = -1$ or $t = 9$\vphantom{$x = -\dfrac{1}{7}$ or $x = 1$}
\task $x = -\dfrac{1}{7}$ or $x = 1$
\task $y = 0$ or $y = \dfrac{2}{\sqrt{2} - 1}$ 
\task $x=1$\vphantom{$w = \dfrac{\sqrt{3} \pm 2}{\sqrt{3} \mp 2}$}
\task $z = -\dfrac{3}{10}$\vphantom{$w = \dfrac{\sqrt{3} \pm 2}{\sqrt{3} \mp 2}$}
\task $w = \dfrac{\sqrt{3} \pm 2}{\sqrt{3} \mp 2}$ 

See footnote\footnote{That is, $w = \dfrac{\sqrt{3} + 2}{\sqrt{3} - 2}$ or $w = \dfrac{\sqrt{3} - 2}{\sqrt{3} + 2}$} 
\task $\left[\dfrac{1}{3}, 3\right]$\vphantom{$\left(-\infty, -\dfrac{12}{7} \right) \cup \left(\dfrac{8}{7}, \infty\right)$}  
\task $\left(-\infty, -\dfrac{12}{7} \right) \cup \left(\dfrac{8}{7}, \infty\right)$
\task $(-3,2)$\vphantom{$\left(-\infty, -\dfrac{12}{7} \right) \cup \left(\dfrac{8}{7}, \infty\right)$}  
\task $(-\infty,1] \cup [3,\infty)$
\task No solution  
\task $(-\infty, \infty)$

\task! $(-\infty, -6-\sqrt{5}) \cup (6-\sqrt{5}, \infty)$ \vphantom{$\left[ -\dfrac{3}{4}, \dfrac{3}{4}\right]$}
\task $\left[ -\dfrac{3}{4}, \dfrac{3}{4}\right]$   

\task No solution 
\task $(-3,2] \cup [6,11)$

\task $[3, 4) \cup (5, 6]$
\task! $\left(\dfrac{2 \sqrt{3} - 3}{2},  \dfrac{2 \sqrt{3} - 1}{2}   \right) \cup \left(\dfrac{2 \sqrt{3} +1}{2},  \dfrac{2 \sqrt{3} +3}{2}   \right)$

\task 
\begin{enumerate}[label=(\alph*)]
    \item $x = -3$, or $x = 1$, or $x = 2$, or $x = 6$
    \item $(-3,1) \cup (2,6)$
\end{enumerate}
\end{tasks}
