\label{ExercisesforAppFactoring}

In Exercises \ref{factoringexfirst} - \ref{factoringexlast}, factor completely over the integers.  Check your answer by multiplication.

\begin{tasks}(2)

\task $2x - 10x^2$ \label{factoringexfirst}
\task $12t^5 - 8t^3$
\task $16xy^2 - 12x^2y$

\task $5(m+3)^2- 4(m+3)^3$
\task $(2x-1)(x+3) - 4(2x-1)$
\task $t^2(t-5) + t - 5$

\task $w^2 - 121$
\task $49 - 4t^2$
\task $81t^4 - 16$

\task $9z^2 - 64y^4$
\task $(y+3)^2 - 4y^2$
\task $(x+h)^3 - (x+h)$

\task $y^2 - 24y + 144$
\task $25t^2 + 10t + 1$
\task $12x^3 - 36x^2 + 27x$

\task $m^4 + 10m^2 + 25$
\task $27 - 8x^3$
\task $t^6 +t^3$

\task $x^2 - 5x - 14$
\task $y^2 - 12y + 27$
\task $3t^2 + 16t + 5$

\task $6x^2 - 23x + 20$
\task $35+2m - m^2$
\task $7w - 2w^2 - 3$

\task $3m^3 + 9m^2 - 12m$
\task $x^4 + x^2 - 20$
\task $4(t^2-1)^2 +3(t^2-1) - 10$
\task $x^3 - 5x^2 - 9x + 45$
\task $3t^2 + t - 3 - t^3$
\task\hspace{-0.1in}\footnote{$y^4 + 5y^2 + 9 = (y^4 + 6y^2 + 9) - y^2$} $y^4 + 5y^2 + 9$\label{factoringexlast}

\end{tasks}

In Exercises \ref{solvebyfactorfirst} - \ref{solvebyfactorlast},  find all rational number solutions.  Check your answers.

\begin{tasks}(2)

\task   $(7x+3)(x-5) = 0$ \label{solvebyfactorfirst}
\task   $(2t-1)^2 (t+4) = 0$
\task   $(y^2 + 4)(3y^2 +y - 10) = 0$

\task   $4t = t^2$
\task   $y+3 = 2y^2$
\task   $26x = 8x^2 + 21$  

\task $16x^4 = 9x^2$
\task $w(6w+11) = 10$
\task $2w^2 + 5w + 2 = - 3(2w+1)$

\task $x^2(x-3) = 16(x-3)$
\task $(2t+1)^3 = (2t+1)$
\task $a^4 + 4 = 6 - a^2$

\task $\dfrac{8t^2}{3} = 2t+3$\vphantom{$\dfrac{y^4}{3} - y^2 = \dfrac{3}{2} (y^2 + 3)$}
\task $\dfrac{x^3+x}{2} = \dfrac{x^2+1}{3}$\vphantom{$\dfrac{y^4}{3} - y^2 = \dfrac{3}{2} (y^2 + 3)$}
\task $\dfrac{y^4}{3} - y^2 = \dfrac{3}{2} (y^2 + 3)$ \label{solvebyfactorlast}

\task!  With help from your classmates, factor $4x^4 + 8x^2 + 9$.  

\task!  With help from your classmates, find an equation which has $3$, $-\frac{1}{2}$, and $117$ as solutions.  

\end{tasks}

\clearpage

\subsection{Answers}

\begin{tasks}(2)

\task $2x(1 - 5x)$ 
\task $4t^3(3t^2-2)$
\task $4xy(4y-3x)$

\task $-(m+3)^2(4m+7)$
\task $(2x-1)(x-1)$
\task $(t-5)(t^2+1)$

\task $(w-11)(w+11)$
\task $(7-2t)(7+2t)$
\task $(3t-2)(3t+2)(9t^2+4)$

\task $(3z-8y^2)(3z+8y^2)$
\task $-3(y - 3)(y+1)$
\task $(x+h)(x+h-1)(x+h+1)$

\task $(y-12)^2$
\task $(5t+1)^2$
\task $3x(2x-3)^2$

\task $(m^2+5)^2$
\task $(3-2x)(9 + 6x + 4x^2)$
\task $t^3(t+1)(t^2 - t + 1)$

\task $(x-7)(x+2)$
\task $(y-9)(y-3)$
\task $(3t+1)(t+5)$

\task $(2x-5)(3x-4)$
\task $(7-m)(5+m)$
\task $(-2w+1)(w-3)$

\task $3m(m-1)(m+4)$
\task $(x-2)(x+2)(x^2+5)$
\task $(2t-3)(2t+3)(t^2+1)$

\task $(x-3)(x+3)(x-5)$
\task $(t-3)(1-t)(1+t)$
\task $(y^2-y+3)(y^2+y+3)$
\task   $x = -\dfrac{3}{7}$ or $x = 5$ 
\task   $t = \dfrac{1}{2}$ or $t = -4$
\task   $y = \dfrac{5}{3}$ or $y = -2$

\task   $t = 0$ or $t = 4$\vphantom{$x = \dfrac{3}{2}$ or $x = \dfrac{7}{4}$ }
\task   $y = -1$ or $y = \dfrac{3}{2}$ \vphantom{$x = \dfrac{3}{2}$ or $x = \dfrac{7}{4}$}
\task   $x = \dfrac{3}{2}$ or $x = \dfrac{7}{4}$ 
\task $x = 0$ or $x = \pm \dfrac{3}{4}$ 
\task $w = -\dfrac{5}{2}$ or $w = \dfrac{2}{3}$
\task $w=-5$ or $w = -\dfrac{1}{2}$

\task $x=3$ or $x = \pm 4$ \vphantom{$t = -1$, $t= -\dfrac{1}{2}$, or $t = 0$}
\task $t = -1$, $t= -\dfrac{1}{2}$, or $t = 0$
\task $a = \pm 1$\vphantom{$t = -1$, $t= -\dfrac{1}{2}$, or $t = 0$}
\task $t = -\dfrac{3}{4}$ or $t = \dfrac{3}{2}$
\task $x = \dfrac{2}{3}$
\task $y = \pm 3$  \vphantom{$x = \dfrac{2}{3}$}

\end{tasks}